vars.thy
@@ -18,8 +18,9 @@ class nat_abs=
   fixes to_nat ::"'a \<Rightarrow> nat"
   fixes subset_nat :: "'a set"
 
-  assumes "a \<in> subset_nat \<Longrightarrow> from_nat (to_nat a) = a "
-  assumes "to_nat (from_nat b) = b"
+  assumes nat_bij:"bij_betw to_nat subset_nat UNIV"
+  assumes abs_nat:"a \<in> subset_nat \<Longrightarrow> from_nat (to_nat a) = a "
+  assumes rep_nat:"to_nat (from_nat b) = b"
 
 class real_abs= nat_abs+
   fixes from_real ::"real \<Rightarrow> 'a"
@@ -31,24 +32,36 @@ class real_abs= nat_abs+
 
 locale vars =  
   fixes variables :: "'v set"
+  fixes types::"'t set"
   fixes v_domain :: "'v \<Rightarrow> ('b::nat_abs) set"
   fixes get_value :: "'s \<Rightarrow> 'v  \<Rightarrow> 'b"
-  fixes set_value ::"'s \<Rightarrow> 'v \<Rightarrow> 'b \<Rightarrow> 's" 
+  (* fixes set_value ::"'s \<Rightarrow> 'v \<Rightarrow> 'b \<Rightarrow> 's"  *)
   fixes conv::"('v \<Rightarrow> 'b) \<Rightarrow> 'v set \<Rightarrow> 's"  
+  fixes is_nat::"'v \<Rightarrow> bool"
 
-  assumes "finite variables"
+  assumes domain_nat:"v \<in> variables \<Longrightarrow> is_nat v \<Longrightarrow> v_domain v = subset_nat"
+  assumes "finite variables" 
   assumes "v \<in> variables \<Longrightarrow> (get_value s v) \<in> v_domain v"
-  assumes eq_get_set:"v \<in> variables \<Longrightarrow> x \<in> (v_domain v) \<Longrightarrow> get_value (set_value s v x) v = x"
+(*  assumes eq_get_set:"v \<in> variables \<Longrightarrow> x \<in> (v_domain v) \<Longrightarrow> get_value (set_value s v x) v = x" *)
   assumes abs_elem: "s = conv (get_value s) variables"
-  
+  assumes get_set:"v \<in> variables \<Longrightarrow> get_value (conv ((get_value s)(v := val)) variables) v = val"
+  (* assumes get_value: "v\<in>variables \<Longrightarrow> 
+                       (get_value (m (v:= x))) = x" *)
+(*  assumes set_value_eq:"set_value s v val = conv (get_value (set_value s v val)) variables" *)
 
+  
 begin
+
+definition set_value:: "'s \<Rightarrow> 'v \<Rightarrow> 'b \<Rightarrow> 's"
+  where "set_value s v val = conv ((get_value s)(v:=val)) variables"
+
+
 
 definition not_access_v::"('s \<Rightarrow> 'n) \<Rightarrow> 'v \<Rightarrow> bool"
 where "not_access_v f v \<equiv>     
   \<forall>s f1 f2. f1 \<in> v_domain v \<and> f2 \<in> v_domain v \<longrightarrow>
-    f (conv ((get_value s)(v:=f1)) variables) = 
-    f (conv ((get_value s)(v:=f2)) variables)" 
+    f (set_value s v f1) = 
+    f (set_value s v f2)" 
 
 definition access_v::"('s \<Rightarrow> 'n) \<Rightarrow> 'v \<Rightarrow> bool"
 where "access_v f v \<equiv>     
@@ -60,7 +73,7 @@ definition not_access_locals::"('s \<Rightarrow> 'n) \<Rightarrow> bool"
 where "not_access_locals f \<equiv> \<forall>v\<in>variables. not_access_v f v"
 
 lemma access_neg:"access_v f v = (\<not> (not_access_v f v))"
-  unfolding access_v_def not_access_v_def by auto
+  unfolding access_v_def not_access_v_def set_value_def by auto
 
 definition modify_v:: "('s \<Rightarrow> 's) \<Rightarrow> 'v \<Rightarrow> bool"
   where "modify_v f v \<equiv> \<exists>s. get_value (f s) v \<noteq> get_value s v"
@@ -70,6 +83,25 @@ definition not_modify_v::"('s \<Rightarrow> 's) \<Rightarrow> 'v \<Rightarrow> b
 
 lemma modify_neg:"modify_v f v =  ( \<not> (not_modify_v f v))" 
   unfolding modify_v_def not_modify_v_def by auto
+
+lemma not_access_v_f_q_eq_set:
+      "q \<in> variables  \<Longrightarrow> 
+       v \<in> v_domain q \<Longrightarrow> 
+       \<sigma>' = set_value \<sigma> q v \<Longrightarrow> 
+       not_access_v f q \<Longrightarrow> f \<sigma> = f \<sigma>'"
+  unfolding not_access_v_def set_value_def 
+  using fun_upd_triv vars_axioms vars_def
+  by metis
+
+lemma from_nat_in_vdomain:
+  assumes a0:"q \<in> variables" and a1:"is_nat q"
+  shows "from_nat q' \<in> v_domain q"
+proof- 
+  have "v_domain q = subset_nat" using domain_nat[OF a0 a1]
+    by auto
+  thus ?thesis using nat_bij abs_nat 
+    by (metis UNIV_I bij_betw_def imageE)
+qed
 
 end
 
